examples/PolyRewrite/Monads/bench/BenchRtac.v
@@ -1,10 +1,15 @@
-Require Import McExamples.Cancel.RtacDemo.
+Require Import McExamples.PolyRewrite.Monads.Monad.
+Require Import McExamples.PolyRewrite.Monads.RtacDemo.
 
-Declare Module M : Monoid.Monoid.
+Declare Module M : Monad.
+Declare Module F : Frob M.
 
-Module Automation := RtacDemo.MonoidCancel M.
+Module Automation := RtacDemo.DemoRtacMonad M F.
 
-Goal Automation.Demo.goal NNN.
+Print Automation.Demo.goal.
+
+Goal Automation.Demo.goal 3.
   Automation.Demo.prep.
-  Time Automation.rtac_canceler.
+  Time Automation.Demo.run.
+  Automation.Demo.cleanup.
 Time Qed.
