examples/PolyRewrite/Monads/bench/run-bench.sh
@@ -2,14 +2,14 @@
 
 FLAGS="-noglob -I ../../../../src -Q ../../../../coq-ext-lib/theories ExtLib -Q ../../.. McExamples -Q ../../../../theories MirrorCore"
 
-for i in 3 5 10 20 50 75 100
+for i in 5 10 15 20 25 30 35
 do
     echo $i
 
     sed "s/NNN/$i/g" BenchLtac.v > BenchLtac$i.v
     sed "s/NNN/$i/g" BenchRtac.v > BenchRtac$i.v
 
-    for t in `seq 1 25`
+    for t in `seq 1 5`
     do
 	coqc  -q  $FLAGS BenchLtac$i | sed -e 's/.*(\(.*\)u,.*/\1/' > ltac.$i.$t.raw
 	coqc  -q  $FLAGS BenchRtac$i | sed -e 's/.*(\(.*\)u,.*/\1/' > rtac.$i.$t.raw
